Generalize AU a lot, AG a bit, write soundness proof

theories/CTree/Logic/AG.v
@@ -31,35 +31,33 @@ Local Open Scope ctree_scope.
 Section BasicLemmas.
   Context {E: Type} {HE: Encode E} {X: Type}.
 
-  Lemma ag_vis: forall e (k: encode e -> ctree E X)
+  Lemma ag_now: forall e (k: encode e -> ctree E X)
                   (v : encode e) w φ,
-      (vis_with φ w /\
-         forall v, <( {k v}, {Obs e v} |= AG vis φ )>) <->
-        <( {Vis e k}, w |= AG vis φ )>.
+      (φ w /\ not_done w /\
+         forall v, <( {k v}, {Obs e v} |= AG now φ )>) <->
+        <( {Vis e k}, w |= AG now φ )>.
   Proof with eauto with ctl.
     split; intros.
-    - destruct H as (Hd & H).
+    - destruct H as (Hφ & Hd & H).
       next; split.
-      + inv Hd...
-        now apply ctl_now.
-      + next; split; inv Hd.
-        * apply can_step_vis... 
-        * intros.
-          apply ktrans_vis in H1 as (i & -> & <- & ?)...
+      + inv Hd.
+        * apply ctl_now...
+        * apply ctl_now...          
+      + cright; apply ax_vis...
     - next in H.
-      destruct H, H0.    
-      apply can_step_not_done in H0. 
-      split...
+      destruct H as ((? & ?) & [? | ?]); try contradiction. 
+      destruct H1.
+      split; [|split]...
       intro v'.
       rewrite unfold_entailsF.
-      apply H1, ktrans_vis...
+      apply H2, ktrans_vis...
   Qed.
   
   Lemma ag_br: forall n (k: fin' n -> ctree E X) w φ,
       (not_done w /\
          forall (i: fin' n), <( {k i}, w |= AG now φ )>) <->
         <( {Br n k}, w |= AG now φ )>.
-  Proof.
+  Proof with auto with ctl.
     split; intros.
     - destruct H as (Hd & H).
       next; split.
@@ -67,20 +65,31 @@ Section BasicLemmas.
         next in H.
         destruct H.
         now cbn in *.
-      + next; split.
+      + right.
+        split.
         * now apply can_step_br.
         * intros.
           apply ktrans_br in H0 as (i & ? & <- & ?).        
           now rewrite H0.
     - next in H.
-      destruct H, H0.     
-      apply can_step_not_done in H0.
-      split; auto.
+      destruct H as ((? & ?) & [? | ?]); try contradiction. 
+      destruct H1.
+      split...
       intro i.
       rewrite unfold_entailsF.
-      apply H1.
+      apply H2.
       apply ktrans_br.
       exists i; auto.
+  Qed.
+
+  Lemma ag_stuck: forall w φ,
+      <( {stuck: ctree E X}, w |= AG φ )> -> False.
+  Proof.
+    intros.
+    remember (stuck) as S.
+    cdestruct H; try contradiction; subst.
+    destruct H0.
+    now apply can_step_stuck in H0.
   Qed.
 
   Lemma ag_ret: forall (x: X) w φ,      
@@ -89,21 +98,14 @@ Section BasicLemmas.
     intros. 
     next in H.
     cdestruct H.
-    next in H0; destruct H0.
-    destruct H0 as (t' & w' & TR).
-    cbn in TR, H1.
-    specialize (H1 _ _ TR).
+    next in H0; cdestruct H0; try contradiction.
+    cdestruct H0.
+    destruct Hs as (S & w' & TR).
+    cbn in TR.
+    specialize (H0 _ _ TR).
     dependent destruction TR; observe_equ x;
-      rewrite <- Eqt, H0 in H1; step in H1; inv H1; try contradiction;
-      destruct H3; apply can_step_not_done in H1; inv H1.
-  Qed.
-
-  Lemma ag_stuck: forall w φ,
-      <( {stuck: ctree E X}, w |= AG now φ )> -> False.
-  Proof.
-    intros.
-    next in H; destruct H, H0.
-    now apply can_step_stuck in H0.
+      rewrite <- Eqt, H0 in H1; cdestruct H1; cdestruct H2; try contradiction;
+      now apply ax_stuck, ag_stuck in H2.
   Qed.
 
   Lemma ag_guard: forall w φ (t: ctree E X),
@@ -161,12 +163,12 @@ Section BindLemmas.
   Qed.
 
   Notation MP X := (rel (ctree E X) (World E)).
-  Program Definition ag_bind_vis_clos{X Y} φ Post : mon (MP Y) :=
+  Program Definition ag_bind_now_clos{X Y} φ Post : mon (MP Y) :=
     {| body R t w :=
         bind_ctx1
-          (fun (t: ctree E X) => <( t, w |= vis φ AU (AX finish Post) )>)
+          (fun (t: ctree E X) => <( t, w |= now φ AU (AX done Post) )>)
           (fun (k: X -> ctree E Y) =>
-             forall (x: X) (e: E) (v: encode e), Post e v x -> R (k x) (Obs e v))
+             forall (x: X) (w: World E), Post x w -> R (k x) w)
           t
     |}.
   Next Obligation.
@@ -175,20 +177,20 @@ Section BindLemmas.
     apply in_bind_ctx1; eauto.
   Qed.
 
-  Lemma ag_bind_vis_ag{X Y} φ Post:
-      ag_bind_vis_clos (X:=X) (Y:=Y) φ Post <= cart <( |- vis φ )> <( |- ⊥ )>.
+  Lemma ag_bind_now_ag{X Y} φ Post:
+      ag_bind_now_clos (X:=X) (Y:=Y) φ Post <= cart <( |- now φ )> <( |- ⊥ )>.
   Proof.    
     apply Coinduction.
     intros R t w; cbn.
     apply (leq_bind_ctx1 _ _
-             (fun t => carF (entailsF <( vis {φ} )>) (entailsF <( ⊥ )>)
-                      (carT (entailsF <( vis {φ} )>) (entailsF <( ⊥ )>)
-                         (ag_bind_vis_clos φ Post) R) t w)). 
+             (fun t => carF (entailsF <( now φ )>) (entailsF <( ⊥ )>)
+                      (carT (entailsF <( now φ )>) (entailsF <( ⊥ )>)
+                         (ag_bind_now_clos φ Post) R) t w)). 
     intros x Hx k Hk.
     cinduction Hx.
     - (* AX done R *)
-      apply ax_done in H as (Hw & x & Heq & e & v & -> & HPost).
-      specialize (Hk _ _ _ HPost); remember (k x) as K;
+      apply ax_done in H as (Hw & x & Heq & HPost).
+      specialize (Hk _ _ HPost); remember (k x) as K;
         destruct Hk; try contradiction; subst.
       apply RStepA.
       + rewrite Heq, bind_ret_l; try (exact (equ eq)); auto.
@@ -196,7 +198,7 @@ Section BindLemmas.
         * rewrite Heq, bind_ret_l.
           now destruct H0.
         * intros t' w' TR.
-          apply (id_T (car_ (entailsF <( vis {φ} )>) (entailsF <( ⊥ )>))); cbn.
+          apply (id_T (car_ (entailsF <( now φ )>) (entailsF <( ⊥ )>))); cbn.
           destruct H0.
           apply H1.
           eapply ktrans_sbisim_ret with (t:=t0); auto.
@@ -208,7 +210,7 @@ Section BindLemmas.
       + apply can_step_bind_l with t' w'; auto.
         destruct (H3 _ _ TR); try contradiction.
         destruct H1.
-        inv H0; constructor.
+        now apply ctl_now in H0.
       + intros k_ w_ TRk.
         apply ktrans_bind_inv in TRk as
             [(t0' & TR0 & Hd_ & Heq) | (x & w0 & TRt0 & Hd & TRk)].
@@ -216,11 +218,11 @@ Section BindLemmas.
           apply (fT_T (mequ_clos_car (KS:=KripkeSetoidEqu))).
           cbn; eapply mequ_clos_ctor with (t1:=x <- t0';; k x) (w1:=w_); auto.
           clear Heq k_.            
-          eapply (fTf_Tf (car_ <( |- vis φ )> <( |- ⊥ )>)).
+          eapply (fTf_Tf (car_ <( |- now φ )> <( |- ⊥ )>)).
           apply in_bind_ctx1.
           -- rewrite unfold_entailsF; auto.             
           -- intros.
-             apply (b_T (car_ <( |- vis φ )> <( |- ⊥ )>)); cbn; auto.
+             apply (b_T (car_ <( |- now φ )> <( |- ⊥ )>)); cbn; auto.
         * (* [t0] steps and is [Ret], contradiction *)
           ddestruction Hd; subst;
             specialize (H3 _ _ TRt0); ddestruction H3;
@@ -233,219 +235,76 @@ Section BindLemmas.
 
   (* [t] satisfies [φ] until it terminates with post-condition [R],
      then forall x w, R x w -> k x, w satisfies [φ] forever. *)
-  Lemma ag_bind_vis{X Y}: forall (t: ctree E X)
+  Lemma ag_bind_r{X Y}: forall (t: ctree E X)
                           w (k: X -> ctree E Y) φ R,
-      <( t, w |= (vis φ) AU (AX finish R) )> ->
-      (forall (x: X) (e: E) (v: encode e), R e v x -> <( {k x}, {Obs e v} |= AG vis φ )>) ->
-      <( {x <- t ;; k x} , w |= AG vis φ )>.
+      <( t, w |= now φ AU AX done R )> ->
+      (forall (x: X) (w: World E), R x w -> <( {k x}, w |= AG now φ )>) ->
+      <( {x <- t ;; k x} , w |= AG now φ )>.
   Proof.
     intros.
     rewrite unfold_entailsF.
-    apply (ft_t (ag_bind_vis_ag φ R)).
+    apply (ft_t (ag_bind_now_ag φ R)).
     cbn.
     apply in_bind_ctx1; auto.
   Qed.
 
-  Lemma ag_iter_vis{X I}: forall (k: I -> ctree E (I + X)) w (x: I) φ R,
+  Lemma ag_iter{X I}: forall (k: I -> ctree E (I + X)) w (x: I) φ R,
       R x ->          (* Iterator invariant: [x] in [R] *)
-      vis_with φ w -> (* Worlds invariant: [w = Obs e v /\ φ e v] *)
-      (forall (i: I) (e: E) (v: encode e),
+      φ w ->          (* Worlds invariant: [φ w] *)
+      not_done w ->
+      (forall (i: I) (w: World E),
           R i ->
-          φ e v ->
-          <( {k i}, {Obs e v} |= AX (vis φ AU AX finish
-                               {fun (e: E) (v: encode e) (lr: I+X) =>
-                                  exists i' : I, lr = inl i' /\ φ e v /\ R i'}))>) ->
-      <( {iter k x}, w |= AG vis φ )>.
+          not_done w ->
+          φ w ->
+          <( {k i}, w |= AX (now φ AU AX done
+                 {fun (lr: I+X) (w: World E) =>
+                    exists i' : I, lr = inl i' /\ φ w /\ not_done w /\ R i'}))>) ->
+      <( {iter k x}, w |= AG now φ )>.
   Proof with auto with ctl.
     (* Coinduction steps *)
     intros.
     generalize dependent x.
     generalize dependent w.    
     coinduction RR CIH; intros.
-    apply RStepA...
-    split; inv H0.
-    - (* can_step (iter k x) w *)
-      specialize (H1 _ _ _ H H2) as HAX.
-      cdestruct HAX.
-      destruct Hs as (k' & w' & TR).
-      rewrite sb_unfold_iter.
-      specialize (HAX _ _ TR); cdestruct HAX.
-      + apply ax_done in H0 as (_ & ? & Heqt & e' & v' & -> & ? & -> & Hφ & HR).                
-        apply can_step_bind_l with t (Obs e' v')...
-      + destruct H3.
-        apply can_step_bind_l with t w...
-        inv H0...
-    - (* coinductive step *)
-      intros t' w' TR.
-      rewrite unfold_iter in TR.
-      apply ktrans_bind_inv in TR as [(t0' & TR0 & Hd_ & Heq) | (x' & w0 & TRt0 & Hd & TRk)].
-      + (* [k x] steps *)
-        rewrite Heq; clear Heq t'.
-        apply (ft_t (ag_bind_vis_ag φ
-                       (fun (e: E) (v: encode e) (lr: I+X) =>
-                          exists i' : I, lr = inl i' /\ φ e v /\ R i'))); cbn.
-        apply in_bind_ctx1.
-        * specialize (H1 _ _ _ H H2) as HAX.
-          cdestruct HAX...
-        * intros [l | r] e' v' (i & Hinv & Hφ & HR); inv Hinv.
-          rewrite sb_guard.
-          apply CIH...
-      + (* [k x] returns *)        
-        specialize (H1 _ _ _ H H2) as HAX.        
+    apply RStepA.
+    - apply ctl_now; auto.
+    - split. 
+      + (* can_step (iter k x) w *)
+        specialize (H2 _ _ H H1 H0) as HAX.
         cdestruct HAX.
-        specialize (HAX _ _ TRt0).
-        apply au_stuck in HAX.
-        cdestruct HAX.
-        now apply can_step_stuck in Hs0.
-  Qed.
-  
-  Program Definition ag_bind_pure_clos{X Y} Post : mon (MP Y) :=
-    {| body R t w :=
-        bind_ctx1
-          (fun (t: ctree E X) => <( t, w |= pure AU AX done {fun x w => Post x /\ w = Pure })>)
-          (fun (k: X -> ctree E Y) => forall (x: X), Post x -> R (k x) Pure)
-          t
-    |}.
-  Next Obligation.
-    revert H0.
-    apply leq_bind_ctx1; intros.
-    apply in_bind_ctx1; eauto.
-  Qed.
-
-  Lemma ag_bind_pure_ag{X Y} Post:
-      ag_bind_pure_clos (X:=X) (Y:=Y) Post <= cart <( |- pure )> <( |- ⊥ )>.
-  Proof.
-    apply Coinduction.
-    intros R t w; cbn.
-    apply (leq_bind_ctx1 _ _
-             (fun t => carF (entailsF <( pure )>) (entailsF <( ⊥ )>)
-                      (carT (entailsF <( pure )>) (entailsF <( ⊥ )>)
-                         (ag_bind_pure_clos Post) R) t w)). 
-    intros x Hx k Hk.
-    cinduction Hx.
-    - (* AX done R *)
-      apply ax_done in H as (Hw & x & Heq & HPost & ->). 
-      specialize (Hk _ HPost); remember (k x) as K;
-        destruct Hk; try contradiction; subst.
-      apply RStepA.
-      + rewrite Heq, bind_ret_l; try (exact (equ eq)); auto.
-      + split.
-        * rewrite Heq, bind_ret_l.
-          now destruct H0.
-        * intros t' w' TR.
-          apply (id_T (car_
-                         (entailsF <( now {fun w0 : World E => w0 = w} )>)
-                         (entailsF <( ⊥ )>))); cbn.
-          destruct H0.
-          apply H1.
-          eapply ktrans_sbisim_ret with (t:=t0); auto.
-    - (* pure *)
-      destruct H0, H1; clear H0.
-      destruct H1 as (t' & w' & TR).
-      apply RStepA; auto.
-      split.
-      + apply can_step_bind_l with t' w'; auto.
-        destruct (H3 _ _ TR); try contradiction.
-        destruct H1.
-        inv H0; constructor.
-      + intros k_ w_ TRk.
-        apply ktrans_bind_inv in TRk as
-            [(t0' & TR0 & Hd_ & Heq) | (x & w0 & TRt0 & Hd & TRk)].
-        * (* [t0] steps and is not [Ret] *)
-          apply (fT_T (mequ_clos_car (KS:=KripkeSetoidEqu))).
-          cbn; eapply mequ_clos_ctor with (t1:=x <- t0';; k x) (w1:=w_); auto.
-          clear Heq k_.            
-          eapply (fTf_Tf (car_ <( |- pure )> <( |- ⊥ )>)).
+        destruct Hs as (k' & w' & TR).
+        rewrite sb_unfold_iter.
+        specialize (HAX _ _ TR); cdestruct HAX.
+        * apply ax_done in H3 as (Hd & y & Hy & i & -> & ? & _ & ?).
+          apply can_step_bind_l with t w0... 
+        * destruct H4.
+          apply can_step_bind_l with t w0...
+          apply ctl_now in H3 as (? & ?)...
+      + (* coinductive step *)
+        intros t' w' TR.
+        rewrite unfold_iter in TR.
+        apply ktrans_bind_inv in TR as
+            [(t0' & TR0 & Hd_ & Heq) | (x' & w0 & TRt0 & Hd & TRk)].
+        * (* [k x] steps *)
+          rewrite Heq; clear Heq t'.
+          apply (ft_t (ag_bind_now_ag φ
+             (fun (lr: I+X) (w0: World E) =>
+                exists i' : I, lr = inl i' /\ φ w0 /\ not_done w0 /\ R i'))); cbn.
           apply in_bind_ctx1.
-          -- rewrite unfold_entailsF; auto.             
-          -- intros.
-             apply (b_T (car_ <( |- pure )> <( |- ⊥ )>)); cbn; auto.
-        * (* [t0] steps and is [Ret], contradiction *)
-          ddestruction Hd; subst;
-            specialize (H3 _ _ TRt0); ddestruction H3;
-            try contradiction;
-            destruct H1, H0;
-            rewrite can_step_bind in H1;
-            destruct H1 as [(? & ? & TRinv & ?) | (? & ? & TRinv & ?)];
-            now apply ktrans_stuck in TRinv.
-  Qed.
-
-  (* [t] satisfies [φ] until it terminates with post-condition [R],
-     then forall x w, R x w -> k x, w satisfies [φ] forever. *)
-  Lemma ag_bind_pure{X Y}: forall (t: ctree E X)
-                          w (k: X -> ctree E Y) R,
-      <( t, w |= pure AU AX done {fun x w => R x /\ w = Pure })> ->
-      (forall (x: X), R x -> <( {k x}, {Pure} |= AG pure )>) ->
-      <( {x <- t ;; k x} , w |= AG pure )>.
-  Proof.
-    intros.
-    rewrite unfold_entailsF.
-    apply (ft_t (ag_bind_pure_ag R)).
-    cbn.
-    apply in_bind_ctx1; auto.
+          -- specialize (H2 _ _ H H1 H0) as HAX.
+             cdestruct HAX...
+          -- intros [l | r] w_ (i & Hinv & Hφ & Hd & HR); inv Hinv.
+             rewrite sb_guard.
+             apply CIH...
+        * (* [k x] returns *)        
+          specialize (H2 _ _ H H1 H0) as HAX.        
+          cdestruct HAX.
+          specialize (HAX _ _ TRt0).
+          apply au_stuck in HAX.
+          cdestruct HAX.
+          now apply can_step_stuck in Hs0.
   Qed.
   
-  Lemma ag_iter_pure{X I}: forall (k: I -> ctree E (I + X)) (x: I) (R: I -> Prop),
-      R x ->          (* Iterator invariant: [x] in [R] *)
-      (forall (i: I),
-          R i ->
-          <( {k i}, Pure |= AX (pure AU AX done
-                               {fun (lr: I+X) (w: World E) =>
-                                  exists i' : I, lr = inl i' /\ R i' /\ w = Pure}))>) ->
-      <( {iter k x}, Pure |= AG pure )>.
-  Proof with auto with ctl.
-    (* Coinduction steps *)
-    intros * HR H.
-    generalize dependent x.
-    coinduction RR CIH; intros.
-    apply RStepA...
-    split.
-    - (* can_step (iter k x) w *)
-      specialize (H _ HR) as HAX.
-      cdestruct HAX.
-      destruct Hs as (k' & w' & TR).
-      rewrite sb_unfold_iter.
-      specialize (HAX _ _ TR); cdestruct HAX.
-      + apply ax_done in H0 as (_ & ? & Heqt & i & -> & HR' & ->). 
-        apply can_step_bind_l with t Pure...
-      + destruct H1.
-        inv H0.
-        apply can_step_bind_l with t Pure...
-    - (* coinductive step *)
-      intros t' w' TR.
-      rewrite unfold_iter in TR.
-      apply ktrans_bind_inv in TR as [(t0' & TR0 & Hd_ & Heq) | (x' & w0 & TRt0 & Hd & TRk)].
-      + (* [k x] steps *)
-        rewrite Heq; clear Heq t'.
-        apply (ft_t (ag_bind_pure_ag
-                       (fun (lr: I+X) => exists i' : I, lr = inl i' /\ R i'))); cbn.
-        apply in_bind_ctx1.
-        * specialize (H _ HR) as HAX.
-          cdestruct HAX.
-          specialize (HAX _ _ TR0).
-          assert(Hdeq:
-                  equiv_ctl (X:= I+X)
-                  <(done {fun (x0 : I + X) (w : World E) =>
-                            (exists i' : I, x0 = inl i' /\ R i') /\ w = Pure})>
-                  <(done {fun (x0 : I + X) (w : World E) =>
-                            exists i' : I, x0 = inl i' /\ R i' /\ w = Pure})>);
-            [|rewrite Hdeq]...
-          split; intros H'; inv H'; destruct H0 as [? Hb].
-          -- destruct H0 as (i & -> & ?); constructor; eauto.
-          -- inv Hb.
-          -- destruct Hb as (-> & ? & ?); constructor; eauto.
-          -- destruct Hb as (-> & ? & Hinv); inv Hinv.
-        * intros ? (i & -> & HR').
-          rewrite sb_guard.
-          apply CIH...
-      + (* [k x] returns *)        
-        specialize (H _ HR) as HAX.        
-        cdestruct HAX.
-        specialize (HAX _ _ TRt0).
-        apply au_stuck in HAX.
-        cdestruct HAX.
-        now apply can_step_stuck in Hs0.
-  Qed.
 End BindLemmas.
 
 (*| Combinators for [interp_state] |*)
@@ -453,7 +312,7 @@ Section CtlAgState.
   Context {E F S: Type} {HE: Encode E} {HF: Encode F}
     (h: E ~> stateT S (ctree F)).
 
-  Theorem ag_bind_state_l{X Y}: forall s w (t: ctree E Y) (k: Y -> ctree E X) φ,
+  Theorem ag_state_bind_l{X Y}: forall s w (t: ctree E Y) (k: Y -> ctree E X) φ,
       <( {interp_state h t s}, w |= AG now φ )> ->
       <( {interp_state h (x <- t ;; k x) s}, w |= AG now φ )>.
   Proof.
@@ -462,76 +321,71 @@ Section CtlAgState.
     now apply ag_bind_l.
   Qed.
 
-  Theorem ag_bind_state_vis{X Y}: forall s (t: ctree E Y) (k: Y -> ctree E X) w φ R,
-      <( {interp_state h t s}, w |= (vis φ) AU (AX finish R) )> ->
-      (forall (e: F) (v: encode e) (y: Y) (s: S),
-          R e v (y, s) ->
-          <( {interp_state h (k y) s}, {Obs e v} |= AG vis φ )>) ->
-      <( {interp_state h (x <- t ;; k x) s} , w |= AG vis φ )>.
+  Theorem ag_state_bind_r{X Y}: forall s (t: ctree E Y) (k: Y -> ctree E X) w φ
+                                  (R: Y -> S -> World F -> Prop),
+      <( {interp_state h t s}, w |= now φ AU (AX done {fun '(x, s) w => R x s w}) )> ->
+      (forall (y: Y) (s: S) (w: World F),
+          R y s w ->
+          <( {interp_state h (k y) s}, w |= AG now φ )>) ->
+      <( {interp_state h (x <- t ;; k x) s} , w |= AG now φ )>.
   Proof.
     intros.
     rewrite interp_state_bind.
-    apply ag_bind_vis with (R:=R); auto.
+    apply ag_bind_r with (R:=fun '(x, s) w => R x s w); auto.
     intros [y s'] w' Hr; auto.
   Qed.
 
-  Theorem ag_bind_state_pure{X Y}: forall s (t: ctree E Y) w (k: Y -> ctree E X) R,
-      <( {interp_state h t s}, w |= pure AU (AX done {fun x w => R x /\ w = Pure}) )> ->
-      (forall (y: Y) (s: S), R (y, s) -> <( {interp_state h (k y) s}, Pure |= AG pure )>) ->
-      <( {interp_state h (x <- t ;; k x) s}, w |= AG pure )>.
-  Proof.
-    intros.
-    rewrite interp_state_bind.
-    apply ag_bind_pure with (R:=R); auto.
-    intros [y s'] Hr; auto.
-  Qed.
-  
-  Theorem ag_iter_state_vis{X I}: forall s (k: I -> ctree E (I + X)) w (x: I) φ R,
-      R (x, s) ->     (* Iterator invariant: [x] in [R] *)
-      vis_with φ w -> (* Worlds invariant: [w = Obs e v /\ φ e v] *)
-      (forall (x: I) (s: S) (e: F) (v: encode e),
-          R (x, s) ->
-          φ e v ->
-          <( {interp_state h (k x) s}, {Obs e v} |= AX (vis φ AU AX finish
-             {fun (e: F) (v: encode e) (lr: (I+X) * S) =>
-                exists (i' : I) (s': S), lr = (inl i', s') /\ φ e v /\ R (i', s')}))>) ->
-      <( {interp_state h (iter k x) s}, w |= AG vis φ )>.
+  Theorem ag_state_iter{X I}: forall s (k: I -> ctree E (I + X)) w (x: I) φ R,
+      R x s ->        (* Iterator invariant: [x] in [R] *)
+      φ w ->          (* Worlds invariant: [φ w] *)
+      not_done w ->
+      (forall (x: I) (s: S) (w: World F),
+          R x s ->
+          φ w ->
+          not_done w ->
+          <( {interp_state h (k x) s}, w |= AX (now φ AU AX done
+             {fun (lr: (I+X) * S) (w: World F) =>
+                exists (i' : I) (s': S), lr = (inl i', s') /\ φ w /\
+                                      not_done w /\ R i' s'}))>) ->
+      <( {interp_state h (iter k x) s}, w |= AG now φ )>.
   Proof with auto with ctl.
     intros.
     rewrite interp_state_unfold_iter.
-    inv H0.
     generalize dependent x.
-    generalize dependent e.
     generalize dependent s.
+    generalize dependent w.
     coinduction RR CIH; intros.
-    apply RStepA; [apply ctl_vis; now constructor|].
+    apply RStepA; [apply ctl_now; now constructor|].
     split.
-    - specialize (H1 _ _ _ _ H H2).
-      cdestruct H1.
+    - (* can_step *)
+      specialize (H2 _ _ _ H H0 H1).
+      cdestruct H2.
       destruct Hs as (t' & w' & TR).
-      specialize (H1 _ _ TR).
+      specialize (H2 _ _ TR).
       apply can_step_bind_l with t' w'; auto.
-      cdestruct H1.
-      + now apply ax_done in H0 as (? & ?).
-      + inv H0; constructor.
+      cdestruct H2.
+      + now apply ax_done in H2 as (? & ?).
+      + now apply ctl_now in H2 as (? & ?). 
     - intros t' w' TR.
-      apply ktrans_bind_inv in TR as [(t0' & TR0 & Hd_ & Heq) | (x' & w0 & TRt0 & Hd & TRk)].
+      apply ktrans_bind_inv in TR as
+          [(t0' & TR0 & Hd_ & Heq) | (x' & w0 & TRt0 & Hd & TRk)].
       + (* [k x] steps *)
         rewrite Heq; clear Heq t'.
-        apply (ft_t (ag_bind_vis_ag φ
-                       (fun (e: F) (v: encode e) (lr: (I+X) * S) =>
-                          exists (i': I) (s': S), lr = (inl i', s') /\ φ e v /\ R (i', s')))); cbn.
+        apply (ft_t (ag_bind_now_ag φ
+                       (fun (lr: (I+X) * S) (w: World F) =>
+                          exists (i': I) (s': S), lr = (inl i', s') /\
+                                               φ w /\ not_done w /\ R i' s'))); cbn.
         apply in_bind_ctx1.
-        * specialize (H1 _ _ _ _ H H2) as HAX.
+        * specialize (H2 _ _ _ H H0 H1) as HAX.
           cdestruct HAX.
           specialize (HAX _ _ TR0).
           apply HAX.
-        * intros (lr' & s_) e' v' (i & s' & Hinv & Hφ & HR'); inv Hinv.
+        * intros (lr' & s_) w_ (i & s' & Hinv & Hφ & Hd' & HR'); inv Hinv.
           rewrite sb_guard.
           setoid_rewrite interp_state_unfold_iter.
           apply CIH...
       + (* [k x] returns *)        
-        specialize (H1 _ _ _ _ H H2) as HAX.        
+        specialize (H2 _ _ _ H H0 H1) as HAX.        
         cdestruct HAX.
         specialize (HAX _ _ TRt0).
         apply au_stuck in HAX.
