theories/CTree/Logic/AF.v
@@ -3,9 +3,6 @@ From Coq Require Import
   Arith.Wf_nat
   Classes.Morphisms.
 
-From Coinduction Require Import
-  coinduction lattice.
-
 From CTree Require Import
   Events.Core
   Events.WriterE
@@ -32,18 +29,6 @@ Local Open Scope ctree_scope.
 Section BasicLemmas.
   Context {E: Type} {HE: Encode E} {X: Type}.
 
-  Lemma au_done: forall (t: ctree E X) ψ φ w,
-      is_done w ->
-      <( t, w |= ψ AU now φ )> ->
-      φ w.
-  Proof.
-    intros * Hret Hcontra.
-    inv Hcontra; auto.
-    destruct H0 as ((? & ? & ?) & ?).
-    exfalso.
-    eapply done_not_ktrans with (t:=t); eauto.
-  Qed.
-
   Lemma au_stuck: forall w φ ψ,
       <( {Ctree.stuck: ctree E X}, w |= φ AU ψ )> <->
         <( {Ctree.stuck: ctree E X}, w |= ψ )>.
@@ -56,47 +41,32 @@ Section BasicLemmas.
     - now next; left.
   Qed.
 
-  Lemma au_ret: forall r w (Rr: rel X (World E)) ψ,      
-      Rr r w ->
-      not_done w ->
-      <( {Ret r}, w |= ψ )> ->
-      <( {Ret r}, w |= ψ AU done Rr )>.
+  Lemma au_ret: forall (r: X) w w' φ ψ,      
+      done_with (fun r' w' => w' = w /\ r' = r) w' ->
+      <( {Ctree.stuck}, w' |= ψ )> ->
+      <( {Ret r}, w |= φ )> ->
+      <( {Ret r}, w |= φ AU ψ )>.
   Proof.
     intros * Hr Hd Hw.
     next; right; split; auto.
     split.
-    - now apply can_step_ret.
+    - apply can_step_ret; inv Hr; intuition. 
     - intros t_ w_ TR_.
-      inv Hd.
-      + cbn in TR_. dependent destruction TR_. 
-        next; left.
-        rewrite ctl_done.
-        now constructor.
+      inv Hr; destruct H as (<- & <-).
+      + apply ktrans_done in TR_ as (-> & ->).
+        next; now left.
       + apply ktrans_finish in TR_ as (-> & ->).
-        next; left.
-        rewrite ctl_done.
-        now constructor.       
+        next; now left.
   Qed.
 
-  Lemma not_done_vis_au: forall (t: ctree E X) φ ψ w,
-      <( t, w |= ψ AU vis φ )> ->
+  Lemma not_done_au: forall (t: ctree E X) φ ψ w,
+      <( t, w |= ψ AU now φ )> ->
       not_done w.
   Proof.
     intros * Hf.
-    next in Hf ; destruct Hf.
-    - inv H; constructor.
-    - destruct H, H0.
-      now apply can_step_not_done with t.
-  Qed.
-
-  Lemma not_done_pure_au: forall (t: ctree E X) w ψ,
-      <( t, w |= ψ AU pure )> ->
-      not_done w.
-  Proof.
-    intros * Hf.
-    next in Hf ; destruct Hf.
-    - subst; constructor. 
-    - destruct H, H0.
+    cdestruct Hf.
+    - now destruct H.
+    - destruct H0.
       now apply can_step_not_done with t.
   Qed.
 
@@ -109,61 +79,60 @@ Section BasicLemmas.
   Qed.
 
   Lemma au_br: forall n (k: fin' n -> ctree E X) w ψ φ,
-      <( {Br n k}, w |= now ψ AU now φ )> <->
-        (forall (i: fin' n), <( {k i}, w |= now ψ AU now φ )>).
+      not_done w ->
+      (<( {Br n k}, w |= φ )> \/
+         <( {Br n k}, w |= ψ )> /\
+           forall (i: fin' n), <( {k i}, w |= ψ AU φ )>) ->
+      <( {Br n k}, w |= ψ AU φ )>.     
   Proof.
-    split; intros.
-    - next in H; cdestruct H.
-      + next; now left. 
-      + cdestruct H.
-        now apply ax_br in H0 as (? & ?).
-    - next.
-      pose proof (H Fin.F1).
-      next in H0; cdestruct H0. 
-      + now left.
-      + cdestruct H0.
-        right; split; auto.
-        split.
-        * apply can_step_br.
-          destruct H1.
-          now apply can_step_not_done with (k Fin.F1).
-        * intros t' w' TR.
-          apply ktrans_br in TR as (i & -> & -> & ?); auto.
+   intros e k * Hd [Hφ | (Hψ & H)].
+   - now next; left. 
+   - next; right; split; auto.
+     next; split.
+     + now apply can_step_br.
+     + intros t' w' TR'.
+       apply ktrans_br in TR' as (? & -> & -> & ?).
+       apply H.
   Qed.
 
-  Lemma au_vis: forall (e: E) (k: encode e -> ctree E X) (_: encode e) w φ ψ,
-      (φ w \/ (ψ w /\ not_done w /\
-                forall (x: encode e), <( {k x}, {Obs e x} |= now ψ AU now φ )>)) ->
-      <( {Vis e k}, w |= now ψ AU now φ )>.        
+  Lemma au_br_inv: forall n (k: fin' n -> ctree E X) w ψ φ,
+      <( {Br n k}, w |= ψ AU φ )> ->
+        (<( {Br n k}, w |= φ )> \/
+          forall (i: fin' n), <( {k i}, w |= ψ AU φ )>).
   Proof.
     intros.
-    destruct H as [H | [Hd H]].
-    - now next; left.
-    - next; right; split; auto.
-      next; split.
-      + now apply can_step_vis.
-      + intros t' w' TR'.
-        apply ktrans_vis in TR' as (? & -> & ? & ?).
-        now rewrite <- H0.
+    next in H; cdestruct H.
+    - now left. 
+    - cdestruct H.
+      right.
+      intros i.        
+      now apply ax_br in H0 as (? & ?).
+  Qed.
+
+  Lemma au_vis_r: forall (e: E) (k: encode e -> ctree E X) w φ ψ,
+      not_done w ->
+      <( {Vis e k}, w |= φ )> ->
+      <( {Vis e k}, w |= ψ AU φ )>.        
+  Proof.
+    intros e k * Hd H. 
+    now next; left.
   Qed.
   
-  Lemma au_vis_done: forall (e: E) (k: encode e -> ctree E X) (_: encode e) w (R: X -> World E -> Prop) ψ,
-      ψ w ->
+  Lemma au_vis_l: forall (e: E) (k: encode e -> ctree E X) (_: encode e) w φ ψ,
       not_done w ->
-      (forall (x: encode e), <( {k x}, {Obs e x} |= now ψ AU AX done R )>) ->
-      <( {Vis e k}, w |= now ψ AU AX done R )>.        
+      <( {Vis e k}, w |= ψ )> ->
+      (forall (x: encode e), <( {k x}, {Obs e x} |= ψ AU φ )>) ->
+      <( {Vis e k}, w |= ψ AU φ )>.        
   Proof.
-    intros.
-    next; right.
-    split.
-    - apply H.
-    - split.
-      + now apply can_step_vis.
-      + intros t' w' TR'.
-        apply ktrans_vis in TR' as (? & -> & <- & ?).
-        apply H1.
+    intros e k wit * Hd Hψ H. 
+    next; right; split; auto.
+    next; split.
+    + now apply can_step_vis.
+    + intros t' w' TR'.
+      apply ktrans_vis in TR' as (? & -> & ? & ?).
+      now rewrite <- H0.
   Qed.
-
+  
   Lemma au_ret_done: forall (x: X) ψ w R,
       <( {Ret x}, w |= now ψ AU (AX done R) )> <->
       (R x w /\ not_done w).
@@ -198,29 +167,30 @@ Section BasicLemmas.
 
 End BasicLemmas.
 
-Section CtlAfBind.
+Section CtlAuBind.
   Context {E: Type} {HE: Encode E}.
 
   Typeclasses Transparent equ.
-  Theorem af_bind_vis{X Y}: forall (t: ctree E Y) (k: Y -> ctree E X) φ w,
-      <( t, w |= AF vis φ )> ->
-      <( {x <- t ;; k x}, w |= AF vis φ )>.
+  Theorem au_bind_l{X Y}: forall (t: ctree E Y) (k: Y -> ctree E X) ψ φ w,
+      <( t, w |= base ψ AU now φ )> ->
+      <( {x <- t ;; k x}, w |= base ψ AU now φ )>.
   Proof.
     intros * Haf.
     revert X k.
-    induction Haf; intros; subst.
+    cinduction Haf; intros; subst.
     - (* MatchA *)
       next; left; cbn.
-      ddestruction H.
-      apply ctl_vis; now constructor.
+      now apply ctl_now. 
     - (* StepA *)
-      destruct H0, H1; clear H H0.      
-      next; right; next; split.
+      destruct H0, H1; clear H1.
+      next; right; split; [|split].
+      + (* now ψ *)
+        apply H.
       + (* can_step *)
-        destruct H1 as (t' & w' & TR').
+        destruct H0 as (t' & w' & TR').
         eapply can_step_bind_l with t' w'; auto.
-        eapply not_done_vis_au with (t:=t') (ψ:=<( ⊤ )>).
-        rewrite !unfold_entailsF.        
+        eapply not_done_au with (t:=t') (ψ:=<( base ψ )>).
+        rewrite unfold_entailsF.        
         now apply H2.
       + (* AX AF *)
         intros t_ w_ TR_.
@@ -229,50 +199,19 @@ Section CtlAfBind.
               (x & w' & TR' & Hr & TRk)].
         * now apply H3.
         * specialize (H2 _ _ TR').
-          inv H2.
-          ddestruction H.
-          -- inv Hr.
-          -- destruct H0.
-             now apply can_step_stuck in H0.
-  Qed.
-
-  Theorem af_bind_pure{X Y}: forall (t: ctree E Y) (k: Y -> ctree E X) w,
-      <( t, w |= AF pure )> ->
-      <( {x <- t ;; k x}, w |= AF pure )>.
-  Proof.
-    intros * Haf.
-    revert X k.
-    cinduction Haf; intros; subst.
-    - (* MatchA *)
-      next; left; cbn.
-      now apply ctl_pure in H. 
-    - (* StepA *)
-      destruct H0, H1; clear H H0.      
-      next; right; next; split.
-      + (* can_step *)
-        destruct H1 as (t' & w' & TR').
-        eapply can_step_bind_l with t' w'; auto.
-        eapply not_done_pure_au with (t:=t') (ψ:=<( ⊤)>).
-        rewrite unfold_entailsF.
-        now apply H2.
-      + (* AX AF *)
-        intros t_ w_ TR_.
-        apply ktrans_bind_inv in TR_.
-        destruct TR_ as [(t' & TR' & Hd & ->) | (x & w' & TR' & Hr & TRk)].
-        * now apply H3.
-        * specialize (H2 _ _ TR').
-          inv H2.
-          apply ctl_pure in H; subst.
-          -- inv Hr.
-          -- destruct H0.
-             now apply can_step_stuck in H0.
+          inv H2; inv Hr;
+            rewrite ctl_base in H, H1.
+          -- destruct H1; inv H2.
+          -- destruct H1; inv H2.
+          -- destruct H4; now apply can_step_stuck in H2.
+          -- destruct H4; now apply can_step_stuck in H2.
   Qed.
 
   Typeclasses Transparent sbisim.
   Lemma au_bind_r{X Y}: forall (t: ctree E Y) (k: Y -> ctree E X) w ψ φ R,
-      <( t, w |= vis ψ AU AX done R )> ->
-      (forall r w', R r w' -> <( {k r}, w' |= vis ψ AU φ )>) ->
-      <( {x <- t ;; k x}, w |= vis ψ AU φ )>.
+      <( t, w |= base ψ AU AX done R )> ->
+      (forall r w', R r w' -> <( {k r}, w' |= base ψ AU φ )>) ->
+      <( {x <- t ;; k x}, w |= base ψ AU φ )>.
   Proof.
     intros.
     cinduction H.
@@ -293,7 +232,7 @@ Section CtlAfBind.
             [(t' & TR' & Hd & ->) | (x & w' & TR' & Hr & TRk)].
         * now apply H4.
         * specialize (H3 _ _ TR').
-          assert(H3': <( {Ctree.stuck: ctree E Y}, w' |= vis ψ AU AX done R)>) by
+          assert(H3': <( {Ctree.stuck: ctree E Y}, w' |= base ψ AU AX done R)>) by
             now rewrite unfold_entailsF.
           apply au_stuck in H3'.
           destruct H3'.
@@ -301,9 +240,9 @@ Section CtlAfBind.
   Qed.
 
   Lemma au_bind_r_eq{X Y}: forall (t: ctree E Y) (k: Y -> ctree E X) w ψ φ r w',
-      <( t, w |= vis ψ AU AX done= r w' )> ->
-      <( {k r}, w' |= vis ψ AU φ )> ->
-      <( {x <- t ;; k x}, w |= vis ψ AU φ )>.
+      <( t, w |= base ψ AU AX done= r w' )> ->
+      <( {k r}, w' |= base ψ AU φ )> ->
+      <( {x <- t ;; k x}, w |= base ψ AU φ )>.
   Proof.
     intros.
     eapply au_bind_r.
@@ -312,70 +251,28 @@ Section CtlAfBind.
       now destruct H1 as (-> & ->). 
   Qed.
 
-  Lemma af_bind_r{X Y}: forall (t: ctree E Y) (k: Y -> ctree E X) w φ R,
-      <( t, w |= AF AX done R )> ->
-      (forall r w', R r w' -> not_done w' -> <( {k r}, w' |= AF φ )>) ->
-      <( {x <- t ;; k x}, w |= AF φ )>.
-  Proof.
-    intros.
-    cinduction H.
-    - apply ax_done in H as (? & ? & ? & HR).
-      rewrite H1, bind_ret_l.
-      now apply H0.
-    - destruct H1, H2; clear H2.
-      next; right; split.
-      + destruct H1 as (t_ & w_ & TR).
-        apply can_step_bind_l with t_ w_; auto.
-        destruct (H3 _ _ TR).
-        * now apply ax_done in H1 as (? & ?).
-        * destruct H2.
-          now apply can_step_not_done with t0.
-      + intros t_ w_ TR.
-        apply ktrans_bind_inv in TR as
-            [(t' & TR' & Hd & ->) | (x & w' & TR' & Hr & TRk)].
-        * now apply H4.
-        * specialize (H3 _ _ TR').
-          assert(H3': <( {Ctree.stuck: ctree E Y}, w' |= AF AX done R)>) by
-            now rewrite unfold_entailsF.
-          apply au_stuck in H3'.
-          destruct H3'.
-          now apply can_step_stuck in H2.
-  Qed.          
+End CtlAuBind.
 
-  Lemma af_bind_r_eq{X Y}: forall (t: ctree E Y) (k: Y -> ctree E X) w φ r w',
-      <( t, w |= AF AX done= r w' )> ->
-      <( {k r}, w' |= AF φ )> ->
-      <( {x <- t ;; k x}, w |= AF φ )>.
-  Proof.
-    intros.
-    eapply af_bind_r.
-    + apply H.
-    + intros.
-      now destruct H1 as (-> & ->). 
-  Qed.
-
-End CtlAfBind.
-
-Section CtlAfIter.
+Section CtlAuIter.
   Context {E: Type} {HE: Encode E}.
 
   (* Total correctness lemma for [iter] *)
   (* [Ri: I -> World E -> Prop] loop invariant (left).
      [Rr: X -> World E -> Prop] loop postcondition (right).
      [Rv: (I * World E) -> (I * World E) -> Prop)] loop variant (left). *)
-  Lemma af_iter{X I} Ri Rr (Rv: relation (I * World E)) (i: I) w (k: I -> ctree E (I + X)):
+  Lemma au_iter{X I} Ri Rr (Rv: relation (I * World E)) (i: I) w (k: I -> ctree E (I + X)) φ:
     (forall (i: I) w,
         Ri i w ->
-        <( {k i}, w |= AF AX done
+        <( {k i}, w |= base φ AU AX done
                     {fun (x: I + X) w' =>
                        match x with
                        | inl i' => Ri i' w' /\
                                     Rv (i', w') (i, w)
-                       | inr r' => Rr r' w'
+                       | inr r' => not_done w' /\ φ w' /\ Rr r' w'
                        end})>) ->
     well_founded Rv ->
     Ri i w ->
-    <( {iter k i}, w |= AF done Rr )>.
+    <( {iter k i}, w |= base φ AU done Rr )>.
   Proof.      
     intros H WfR Hi.
     generalize dependent k.
@@ -384,151 +281,121 @@ Section CtlAfIter.
     replace i with (fst P) by now subst.
     replace w with (snd P) by now subst.
     clear HeqP i w.
-    Opaque entailsF.
     induction P using (well_founded_induction WfR);
       destruct P as (i, w); cbn in *. 
     rename H into HindWf.
     intros.
     unfold iter, MonadIter_ctree.
     rewrite unfold_iter.
-    eapply af_bind_r with
+    eapply au_bind_r with
       (R:=fun (x : I + X) (w' : World E) =>
             match x with
             | inl i' => Ri i' w' /\ Rv (i', w') (i, w)
-            | inr r' => Rr r' w'
+            | inr r' => not_done w' /\ φ w' /\ Rr r' w'
             end); auto.
-    intros [i' | r] w'.
-    - intros (Hi' & Hv) Hd.
+    intros [i' | r] w'.            
+    - intros (Hi' & Hv). 
       apply au_guard.
       remember (i', w') as y.
       replace i' with (fst y) by now subst.
       replace w' with (snd y) by now subst.      
       apply HindWf; inv Heqy; auto.
-    - intros HR Hd; apply au_ret; auto.
+    - intros [Hd HR]; inv Hd.
+      + apply au_ret with (w':=Done r); auto with ctl.
+        * apply ctl_done; now constructor.
+        * apply ctl_base; intuition. 
+      + apply au_ret with (w':=Finish e v r); auto with ctl.
+        * apply ctl_done; now constructor.
+        * apply ctl_base; intuition. 
   Qed.
 
-  (*| Instead of a WF relation [Rv] provide a "ranking" function [f] |*)
-  Lemma af_iter_nat{X I} Ri Rr (f: I -> World E -> nat) (i: I) w (k: I -> ctree E (I + X)):
+  (*| Instead of a WF relation [Rv] a "ranking" function [f] |*)
+  Lemma au_iter_nat{X I} Ri Rr (f: I -> World E -> nat) (i: I) w (k: I -> ctree E (I + X)) φ:
     (forall (i: I) w,
         Ri i w ->
-        <( {k i}, w |= AF AX done
+        <( {k i}, w |= base φ AU AX done
                     {fun (x: I + X) w' =>
                        match x with
                        | inl i' => Ri i' w' /\ f i' w' < f i w
-                       | inr r' => Rr r' w'
+                       | inr r' => not_done w' /\ φ w' /\ Rr r' w'
                        end})>) ->
     Ri i w ->
-    <( {iter k i}, w |= AF done Rr )>.
+    <( {iter k i}, w |= base φ AU done Rr )>.
   Proof.
     intros.
-    eapply af_iter with Ri (ltof _ (fun '(i, w) => f i w));
+    eapply au_iter with Ri (ltof _ (fun '(i, w) => f i w));
       auto.
     apply well_founded_ltof.
   Qed.
 
-  Lemma af_iter_nat'{X I} Rr (f: I -> World E -> nat) (i: I) w (k: I -> ctree E (I + X)):
-    (forall (i: I) w,
-        not_done w ->
-        <( {k i}, w |= AF AX done
-                    {fun (x: I + X) w' =>
-                       match x with
-                       | inl i' => not_done w' /\ f i' w' < f i w
-                       | inr r' => Rr r' w'
-                       end})>) ->
-    not_done w ->
-    <( {iter k i}, w |= AF done Rr )>.
-  Proof.
-    intros.
-    eapply af_iter_nat with
-      (Ri:=fun _ => not_done) (f:=f); intros; auto.
-  Qed.
-
   (* Well-founded induction on length of lists *)
-  Lemma af_iter_list{A X I} Ri Rr (f: I -> World E -> list A) (i: I) w (k: I -> ctree E (I + X)):
+  Lemma au_iter_list{A X I} Ri Rr (f: I -> World E -> list A) (i: I) w (k: I -> ctree E (I + X)) φ:
     (forall (i: I) w,
         Ri i w ->
-        <( {k i}, w |= AF AX done
+        <( {k i}, w |= base φ AU AX done
                     {fun (x: I + X) w' =>
                        match x with
                        | inl i' => Ri i' w' /\ length (f i' w') < length (f i w)
-                       | inr r' => Rr r' w'
+                       | inr r' => not_done w' /\ φ w' /\ Rr r' w'
                        end})>) ->
     Ri i w ->
-    <( {iter k i}, w |= AF done Rr )>.
+    <( {iter k i}, w |= base φ AU done Rr )>.
   Proof.
     intros.
-    eapply af_iter_nat with
+    eapply au_iter_nat with
       Ri (fun i w => length (f i w)); auto.
   Qed.
-
-  Lemma af_iter_list'{A X I} Rr (f: I -> World E -> list A) (i: I) w (k: I -> ctree E (I + X)):
-    (forall (i: I) w,
-        not_done w ->
-        <( {k i}, w |= AF AX done
-                    {fun (x: I + X) w' =>
-                       match x with
-                       | inl i' => not_done w' /\
-                                    length (f i' w') < length (f i w)
-                       | inr r' => Rr r' w'
-                       end})>) ->
-    not_done w ->
-    <( {iter k i}, w |= AF done Rr )>.
-  Proof.
-    intros.
-    eapply af_iter_list with
-      (Ri:=fun _ => not_done) (f:=f); intros; auto.
-  Qed.  
-End CtlAfIter.
+End CtlAuIter.
 
 (*| Combinators for [interp_state] |*)
-Section CtlAfState.
+Section CtlAuState.
   Context {E F S: Type} {HE: Encode E} {HF: Encode F}
     (h: E ~> stateT S (ctree F)).
 
-  Theorem af_bind_state_vis{X Y}: forall s w (t: ctree E Y) (k: Y -> ctree E X) φ,
-      <( {interp_state h t s}, w |= AF vis φ )> ->
-      <( {interp_state h (x <- t ;; k x) s}, w |= AF vis φ )>.
-  Proof.
-    intros.
-    rewrite interp_state_bind.
-    now apply af_bind_vis.
-  Qed.
-  
-  Theorem af_bind_state_pure{X Y}: forall s w (t: ctree E Y) (k: Y -> ctree E X),
-      <( {interp_state h t s}, w |= AF pure )> ->
-      <( {interp_state h (x <- t ;; k x) s}, w |= AF pure )>.
-  Proof.
-    intros.
-    rewrite interp_state_bind.
-    now apply af_bind_pure.
-  Qed.
-
-  Theorem af_bind_state_r{X Y}: forall s (t: ctree E Y) (k: Y -> ctree E X) w φ (R: Y * S -> World F -> Prop),
-      <( {interp_state h t s}, w |= AF AX done R )> ->
-      (forall (y: Y) (s: S) w, R (y,s) w ->
-                    not_done w ->
-                    <( {interp_state h (k y) s}, w |= AF now φ )>) ->
+  Theorem au_state_bind_l{X Y}: forall s w (t: ctree E Y) (k: Y -> ctree E X) φ,
+      <( {interp_state h t s}, w |= AF now φ )> ->
       <( {interp_state h (x <- t ;; k x) s}, w |= AF now φ )>.
   Proof.
     intros.
     rewrite interp_state_bind.
-    apply af_bind_r with (R:=R); auto.
-    intros [y s'] w' Hr Hd; auto.
+    now apply au_bind_l.
+  Qed.  
+
+  Theorem au_state_bind_r{X Y}: forall s (t: ctree E Y) (k: Y -> ctree E X) w ψ φ (R: Y * S -> World F -> Prop),
+      <( {interp_state h t s}, w |= base ψ AU AX done R )> ->
+      (forall (y: Y) (s: S) w, R (y,s) w ->
+          <( {interp_state h (k y) s}, w |= base ψ AU φ )>) ->
+      <( {interp_state h (x <- t ;; k x) s}, w |= base ψ AU φ )>.
+  Proof.
+    intros.
+    rewrite interp_state_bind.
+    apply au_bind_r with (R:=R); auto.
+    intros [y s'] w' Hr; auto.
   Qed.
-     
-  Theorem af_iter_state{X I} s Ri (Rr: rel (X * S) (World F))  Rv (i: I) (k: I -> ctree E (I + X)) w:
+
+  Theorem au_state_bind_r_eq{X Y}: forall s s' (t: ctree E Y) (k: Y -> ctree E X) w w' ψ φ (r: Y),
+      <( {interp_state h t s}, w |= base ψ AU AX done={(r, s')} w' )> ->
+      <( {interp_state h (k r) s'}, w' |= base ψ AU φ )> ->
+      <( {interp_state h (x <- t ;; k x) s}, w |= base ψ AU φ )>.
+  Proof.
+    intros.
+    rewrite interp_state_bind.
+    apply au_bind_r_eq with (r, s') w'; auto. 
+  Qed.
+
+  Theorem au_state_iter{X I} s Ri (Rr: rel (X * S) (World F)) Rv (i: I) (k: I -> ctree E (I + X)) φ w:
     (forall (i: I) w s,
         Ri i w s ->
-        <( {interp_state h (k i) s}, w |= AF AX done
+        <( {interp_state h (k i) s}, w |= base φ AU AX done
           {fun '(x, s') w' =>
              match x with
              | inl i' => Ri i' w' s'
                         /\ Rv (i', w', s') (i, w, s)
-             | inr r' => Rr (r',s') w'
+             | inr r' => not_done w' /\ φ w' /\ Rr (r',s') w'
              end})>) ->
     well_founded Rv ->
     Ri i w s ->
-    <( {interp_state h (Ctree.iter k i) s}, w |= AF done Rr )>.
+    <( {interp_state h (Ctree.iter k i) s}, w |= base φ AU done Rr )>.
   Proof.
     intros H WfR Hi.
     generalize dependent k.
@@ -538,99 +405,70 @@ Section CtlAfState.
     replace w with (snd (fst P)) by now subst.
     replace s with (snd P) by now subst.
     clear HeqP i w s.
-    Opaque entailsF.
     induction P using (well_founded_induction WfR);
       destruct P as ((i, w), s); cbn in *. 
     rename H into HindWf.
     intros.
     rewrite interp_state_unfold_iter.
-    eapply af_bind_r with (R:=fun '(r, s0) (w0 : World F) =>
+    eapply au_bind_r with (R:=fun '(r, s0) (w0 : World F) =>
                       match r with
                       | inl i' => Ri i' w0 s0 /\ Rv (i', w0, s0) (i, w, s)
-                      | inr r' => Rr (r',s0) w0
+                      | inr r' => not_done w0 /\ φ w0 /\ Rr (r',s0) w0
                       end); auto.
     intros ([i' | r] & s') w'; cbn.
-    - intros (Hi' & Hv) Hd.
+    - intros (Hi' & Hv).
       apply au_guard.
       remember (i', w',s') as y.
       replace i' with (fst (fst y)) by now subst.
       replace w' with (snd (fst y)) by now subst.
       replace s' with (snd y) by now subst.      
       apply HindWf; inv Heqy; auto.
-    - intros; apply au_ret; auto.
+    - intros (Hd & HR & Hr); inv Hd.
+      + apply au_ret with (w':=Done (r, s')); auto with ctl.
+        apply ctl_done; now constructor.
+      + apply au_ret with (w':=Finish e v (r,s')); auto with ctl.
+        apply ctl_done; now constructor.
   Qed.
     
-  (*| Instead of a WF relation [Rv] provide a "ranking" function [f] |*)
-  Lemma af_iter_state_nat{X I} (s: S) Ri (Rr: rel (X * S) (World F)) (f: I -> World F -> S -> nat) (i: I) w
+  (*| Instead of a WF relation [Rv] a "ranking" function [f] |*)
+  Lemma au_state_iter_nat{X I} (s: S) Ri (Rr: rel (X * S) (World F)) (f: I -> World F -> S -> nat) (i: I) φ w
     (k: I -> ctree E (I + X)):
     (forall (i: I) w s,
         Ri i w s ->
-        <( {interp_state h (k i) s}, w |= AF AX done
+        <( {interp_state h (k i) s}, w |= base φ AU AX done
                     {fun '(x, s') w' =>
                        match x with
                        | inl i' => Ri i' w' s' /\ f i' w' s' < f i w s
-                       | inr r' => Rr (r',s') w'
+                       | inr r' => not_done w' /\ φ w' /\ Rr (r',s') w'
                        end})>) ->
     Ri i w s ->
-    <( {interp_state h (Ctree.iter k i) s}, w |= AF done Rr )>.
+    <( {interp_state h (Ctree.iter k i) s}, w |= base φ AU done Rr )>.
   Proof.
     intros.
-    eapply af_iter_state with Ri (ltof _ (fun '(i, w, s) => f i w s)); auto.
+    eapply au_state_iter with Ri (ltof _ (fun '(i, w, s) => f i w s)); auto.
     apply well_founded_ltof.
   Qed.
 
-  Lemma af_iter_state_nat'{X I} (Rr: rel (X * S) (World F)) (f: I -> S -> nat) (s: S)
-    (i: I) w (k: I -> ctree E (I + X)):
-    (forall (i: I) w s,
-        not_done w ->
-        <( {interp_state h (k i) s}, w |= AF AX done
-                    {fun '(x, s') w' =>
-                       match x with
-                       | inl i' => not_done w' /\ f i' s' < f i s
-                       | inr r' => Rr (r',s') w'
-                       end})>) ->
-    not_done w ->
-    <( {interp_state h (Ctree.iter k i) s}, w |= AF done Rr )>.
-  Proof.
-    intros.
-    eapply af_iter_state_nat with (Ri:=fun _ w _ => not_done w) (f:=fun i _ => f i); auto.
-  Qed.
-End CtlAfState.
+End CtlAuState.
 
 (*| Combinators for [interp_state] with [writerE] |*)
-Section CtlAfStateList.
+Section CtlAuStateList.
   Context {E F A: Type} {HE: Encode E} {HF: Encode F} (h: E ~> stateT (list A) (ctree F)).
 
-  Lemma af_iter_state_list{X I} Ri (Rr: rel (X * list A) (World F)) (l: list A) w (i: I) (k: I -> ctree E (I + X)):
+  Lemma au_state_iter_list{X I} Ri (Rr: rel (X * list A) (World F)) (l: list A) w (i: I) (k: I -> ctree E (I + X)) φ :
     (forall (i: I) w (l: list A),
         Ri i w l ->
-        <( {interp_state h (k i) l}, w |= AF AX done
+        <( {interp_state h (k i) l}, w |= base φ AU AX done
                  {fun '(x, l') w' =>
                     match x with
                     | inl i' => Ri i' w' l' /\ length l' < length l
-                    | inr r' => Rr (r', l') w'
+                    | inr r' => not_done w' /\ φ w' /\ Rr (r', l') w'
                     end})>) ->
     Ri i w l ->
-    <( {interp_state h (Ctree.iter k i) l}, w |= AF done Rr )>.
+    <( {interp_state h (Ctree.iter k i) l}, w |= base φ AU done Rr )>.
   Proof.
     intros.
-    apply af_iter_state_nat with (Ri:=Ri) (f:=fun _ _ l => length l); auto.
+    apply au_state_iter_nat with (Ri:=Ri) (f:=fun _ _ l => length l);
+      auto.
   Qed.
-
-  Lemma af_iter_state_list'{X I} (Rr: rel (X * list A) (World F)) (l: list A) (i: I) w (k: I -> ctree E (I + X)):
-    (forall (i: I) w (l: list A),
-        not_done w ->
-        <( {interp_state h (k i) l}, w |= AF AX done
-             {fun '(x, l') w' =>
-                match (x: I + X) with
-                | inl _ => not_done w' /\ length l' < length l
-                | inr r' => Rr (r',l') w'
-                end})>) ->
-    not_done w ->
-    <( {interp_state h (Ctree.iter k i) l}, w |= AF done Rr )>.
-  Proof.
-    intros.
-    eapply af_iter_state_list with (Ri:=fun _ w _ => not_done w); auto.
-  Qed.
-
-End CtlAfStateList.  
+End CtlAuStateList.
