theories/CTree/Logic/Soundness.v
@@ -1,0 +1,117 @@
+From Coq Require Import
+  Basics
+  Classes.Morphisms.
+
+From CTree Require Import
+  Events.Core
+  Events.WriterE
+  CTree.Core
+  CTree.Equ
+  CTree.SBisim
+  CTree.Interp.Core
+  CTree.Interp.State
+  CTree.Logic.Trans
+  CTree.Logic.CanStep
+  Logic.Ctl
+  Logic.AX
+  Logic.AF
+  Logic.Kripke
+  Logic.Setoid.
+
+Set Implicit Arguments.
+Generalizable All Variables.
+
+Import CTreeNotations CtlNotations.
+Local Open Scope ctl_scope.
+Local Open Scope ctree_scope.
+
+Section SyntacticEntailment.
+  Context {E: Type} {HE: Encode E}.
+
+  Inductive syntails{X}: ctree E X -> World E -> ctlf E X -> Prop :=
+  (* All formulas are invariant to [Guard] *)
+  | SynGuard: forall w φ t,
+      syntails t w φ ->
+      syntails (Guard t) w φ
+  (* Base predicates (ignore t) *)
+  | SynNow: forall w φ t,
+      φ w ->
+      syntails t w <( base φ )>
+  | SynDone: forall w φ t,
+      done_with φ w ->
+      syntails t w <( done φ )>
+  (* ψ AU φ *)
+  | SynAuStuck: forall w φ ψ,
+    syntails (Ctree.stuck) w ψ ->
+    syntails (Ctree.stuck) w <( φ AU ψ )>
+  | SynAuRet: forall w w' φ ψ r,
+      done_with (fun r' w' => w' = w /\ r' = r) w' ->
+      syntails (Ctree.stuck) w' <( ψ )> ->
+      syntails (Ret r) w <( φ )> ->
+      syntails (Ret r) w <( φ AU ψ )>
+  | SynAuBrR: forall w n (k: fin' n -> _) φ ψ,
+      not_done w ->
+      syntails (Br n k) w φ ->
+      syntails (Br n k) w <( ψ AU φ )>
+  | SynAuBrL: forall w n (k: fin' n -> _) φ ψ,
+      not_done w ->      
+      syntails (Br n k) w ψ ->
+      (forall (i: fin' n), syntails (k i) w <( ψ AU φ )>) ->
+      syntails (Br n k) w <( ψ AU φ )>
+  | SynAuVisR: forall w (e: E) (k: encode e -> _) φ ψ,
+      not_done w ->
+      syntails (Vis e k) w φ ->
+      syntails (Vis e k) w <( ψ AU φ )>
+  | SynAuVisL: forall w (e: E) (k: encode e -> _) (wit: encode e) φ ψ,
+      not_done w ->
+      syntails (Vis e k) w ψ ->
+      (forall (x: encode e), syntails (k x) (Obs e x) <( ψ AU φ )>) ->
+      syntails (Vis e k) w <( ψ AU φ )>
+  | SynAuBindL: forall {Y} (t: ctree E Y) (k: Y -> ctree E X) φ ψ w,
+      syntails t w <(base φ AU now ψ )> ->
+      syntails (x <- t ;; k x) w <( base φ AU now ψ )>
+  | SynAuBindR: forall {Y} (t: ctree E Y) (k: Y -> ctree E X) w ψ φ R,
+      syntails t w <( base ψ AU AX done R )> ->
+      (forall r w', R r w' -> syntails (k r)  w' <( base ψ AU φ )>) ->
+      syntails (x <- t ;; k x) w <( base ψ AU φ )>
+  | SynAuIter: forall {I} Ri Rr Rv (i: I) w (k: I -> ctree E (I + X)) φ,
+      (forall (i: I) w,
+          Ri i w ->
+          syntails (k i) w <( base φ AU AX done
+                      {fun (x: I + X) w' =>
+                         match x with
+                         | inl i' => Ri i' w' /\
+                                      Rv (i', w') (i, w)
+                         | inr r' => not_done w' /\ φ w' /\ Rr r' w'
+                         end})>) ->
+      well_founded Rv ->
+      Ri i w ->
+      syntails (iter k i) w <( base φ AU done Rr )>.
+  
+  (* Define a second "deterministic entailment" for this 
+  | SynAuBindDetR: forall {Y} (t: ctree E Y)
+                   (k: Y -> ctree E X) w w' r ψ φ,
+      syntails t w <( vis ψ AU AX done= r w' )> ->
+      syntails (k r)  w' <( vis ψ AU φ )> ->
+      syntails (x <- t ;; k x) w <( vis ψ AU φ )>. *)
+
+  Lemma soundness{X}: forall (t: ctree E X) (w: World E) (φ: ctlf E X),
+      syntails t w φ -> <( t, w |= φ )>.
+  Proof with auto with ctl.
+    intros.
+    induction H.
+    - rewrite sb_guard...
+    - apply ctl_base...
+    - apply ctl_done...
+    - apply au_stuck...
+    - apply au_ret with w'...
+    - apply au_br...
+    - apply au_br...
+    - apply au_vis_r... 
+    - apply au_vis_l...
+    - apply au_bind_l...
+    - apply au_bind_r with (R:=R)...
+    - apply au_iter with Ri Rv...
+  Qed.
+End SyntacticEntailment.
+    
